DY/Actions/PersistentLocalState.lean
@@ -49,7 +49,7 @@ grind_pattern LocalState.IsWellFormed_eq => Comparse.IsWellFormed pre x tr
 
 namespace State
 
-@[expose]
+@[expose, reducible]
 public
 def ExecEntryT.internal (StateT: Type): Fin 1 → Type
   | 0 => PersistentGlobalState.State.ExecEntryT (LocalState StateT)
@@ -98,7 +98,7 @@ end Execution
 section Proof
 
 public
-class LocalStateInv [TraceTypes] (StateT: Type) where
+class LocalStateInv [ExecTraceTypes] [ProofTraceTypes] (StateT: Type) where
   invariant: Participant → StateT → ProofTrace → Prop
   invariant_later: ∀ p st tr1 tr2,
     tr1 ≤ tr2 →
@@ -117,7 +117,7 @@ def ProofEntryT.internal (StateT: Type): Fin 1 → Type
 
 public
 abbrev ProofEntryT (StateT: Type): Type :=
-  TraceTypes.combine (ProofEntryT.internal StateT)
+  ProofTraceTypes.combine (ProofEntryT.internal StateT)
 
 public
 instance (StateT: Type): ∀ id, ErasableProofEntry (ExecEntryT.internal StateT id) (ProofEntryT.internal StateT id)
@@ -125,15 +125,15 @@ instance (StateT: Type): ∀ id, ErasableProofEntry (ExecEntryT.internal StateT 
 
 public
 instance (StateT: Type): ErasableProofEntry (ExecEntryT StateT) (ProofEntryT StateT) :=
-  (inferInstance: ErasableProofEntry (ExecTraceTypes.combine (ExecEntryT.internal StateT)) (TraceTypes.combine (ProofEntryT.internal StateT)))
+  (inferInstance: ErasableProofEntry (ExecTraceTypes.combine (ExecEntryT.internal StateT)) (ProofTraceTypes.combine (ProofEntryT.internal StateT)))
 
 public
-instance (StateT: Type): TraceTypes.HasStep (PersistentGlobalState.State.ProofEntryT (LocalState StateT)) (ProofEntryT StateT) :=
-  inferInstanceAs (TraceTypes.HasStep (ProofEntryT.internal StateT 0) (TraceTypes.combine (ProofEntryT.internal StateT)))
+instance (StateT: Type): ProofTraceTypes.HasStep (PersistentGlobalState.State.ProofEntryT (LocalState StateT)) (ProofEntryT StateT) :=
+  inferInstanceAs (ProofTraceTypes.HasStep (ProofEntryT.internal StateT 0) (ProofTraceTypes.combine (ProofEntryT.internal StateT)))
 
 public
 instance
-  [TraceTypes]
+  [ExecTraceTypes] [ProofTraceTypes]
   (StateT: Type) [LocalStateInv StateT]
   : PersistentGlobalState.GlobalStateInv (LocalState StateT)
 where
@@ -141,23 +141,24 @@ where
   invariant_later st tr1 tr2 := LocalStateInv.invariant_later st.participant st.state tr1 tr2
 
 public
-instance [TraceTypes] (StateT: Type) [LocalStateInv StateT]: ∀ id, SubTraceInvariant (ProofEntryT.internal StateT id)
+instance [ExecTraceTypes] [ProofTraceTypes] (StateT: Type) [LocalStateInv StateT]: ∀ id, SubTraceInvariant (ProofEntryT.internal StateT id)
   | 0 => by dsimp only [ProofEntryT.internal]; infer_instance
 
 public
-instance [TraceTypes] (StateT: Type) [LocalStateInv StateT]: SubTraceInvariant (ProofEntryT StateT) :=
-  (inferInstance: SubTraceInvariant (TraceTypes.combine (ProofEntryT.internal StateT)))
+instance [ExecTraceTypes] [ProofTraceTypes] (StateT: Type) [LocalStateInv StateT]: SubTraceInvariant (ProofEntryT StateT) :=
+  (inferInstance: SubTraceInvariant (ProofTraceTypes.combine (ProofEntryT.internal StateT)))
 
 public
-instance [TraceTypes] (StateT: Type) [LocalStateInv StateT]: TraceInvariant.HasStep (PersistentGlobalState.State.ProofEntryT (LocalState StateT)) (ProofEntryT StateT) :=
-  inferInstanceAs (TraceInvariant.HasStep (ProofEntryT.internal StateT 0) (TraceTypes.combine (ProofEntryT.internal StateT)))
+instance [ExecTraceTypes] [ProofTraceTypes] (StateT: Type) [LocalStateInv StateT]: TraceInvariant.HasStep (PersistentGlobalState.State.ProofEntryT (LocalState StateT)) (ProofEntryT StateT) :=
+  inferInstanceAs (TraceInvariant.HasStep (ProofEntryT.internal StateT 0) (ProofTraceTypes.combine (ProofEntryT.internal StateT)))
 
 public
 instance
-  [TraceInvariant] [BytesFunctor] [BytesInvariants]
+  [ExecTraceTypes] [ProofTraceTypes] [TraceInvariant] [BytesFunctor] [BytesInvariants]
   (StateT: Type)
   [LocalStateInv StateT]
-  [TraceTypes.Has (ProofEntryT StateT)]
+  [ExecTraceTypes.Has (ExecEntryT StateT)]
+  [ProofTraceTypes.Has (ProofEntryT StateT)]
   [TraceInvariant.Has (ProofEntryT StateT)]
   : ∀ id, SubBaseAttackerKnowledgeTheorem (ProofEntryT.internal StateT id) (baseAttackerKnowledge.internal StateT id)
   -- TODO: investigate why infer_instance doesn't work
@@ -165,10 +166,11 @@ instance
 
 public
 instance baseAttackerKnowledgeTheorem
-  [TraceInvariant] [BytesFunctor] [BytesInvariants]
+  [ExecTraceTypes] [ProofTraceTypes] [TraceInvariant] [BytesFunctor] [BytesInvariants]
   (StateT: Type)
   [LocalStateInv StateT]
-  [TraceTypes.Has (ProofEntryT StateT)]
+  [ExecTraceTypes.Has (ExecEntryT StateT)]
+  [ProofTraceTypes.Has (ProofEntryT StateT)]
   [TraceInvariant.Has (ProofEntryT StateT)]
   : SubBaseAttackerKnowledgeTheorem (ProofEntryT StateT) (baseAttackerKnowledge StateT)
 := by
@@ -181,9 +183,9 @@ end State
 public
 theorem storeLocalState.spec
   {StateT: Type}
-  [TraceInvariant]
+  [ExecTraceTypes] [ProofTraceTypes] [TraceInvariant]
   [LocalStateInv StateT]
-  [TraceTypes.Has (State.ProofEntryT StateT)] [TraceInvariant.Has (State.ProofEntryT StateT)]
+  [ExecTraceTypes.Has (State.ExecEntryT StateT)] [ProofTraceTypes.Has (State.ProofEntryT StateT)] [TraceInvariant.Has (State.ProofEntryT StateT)]
   (participant: Participant) (state: StateT)
   : HoareTriple
     (storeLocalState participant state)
@@ -199,9 +201,9 @@ theorem storeLocalState.spec
 public
 theorem getLocalState.spec
   {StateT: Type}
-  [TraceInvariant]
+  [ExecTraceTypes] [ProofTraceTypes] [TraceInvariant]
   [LocalStateInv StateT]
-  [TraceTypes.Has (State.ProofEntryT StateT)] [TraceInvariant.Has (State.ProofEntryT StateT)]
+  [ExecTraceTypes.Has (State.ExecEntryT StateT)] [ProofTraceTypes.Has (State.ProofEntryT StateT)] [TraceInvariant.Has (State.ProofEntryT StateT)]
   (participant: Participant) (i: Nat)
   : HoareTriple
     (getLocalState participant i: Traceful StateT)
@@ -306,7 +308,7 @@ def ProofEntryT.internal (StateT: Type): Fin 1 → Type
 @[expose, implicit_reducible]
 public
 def ProofEntryT (StateT: Type): Type :=
-  TraceTypes.combine (ProofEntryT.internal StateT)
+  ProofTraceTypes.combine (ProofEntryT.internal StateT)
 
 public
 instance (StateT: Type): ∀ id, ErasableProofEntry (ExecEntryT.internal StateT id) (ProofEntryT.internal StateT id)
@@ -314,29 +316,30 @@ instance (StateT: Type): ∀ id, ErasableProofEntry (ExecEntryT.internal StateT 
 
 public
 instance (StateT: Type): ErasableProofEntry (ExecEntryT StateT) (ProofEntryT StateT) :=
-  (inferInstance: ErasableProofEntry (ExecTraceTypes.combine (ExecEntryT.internal StateT)) (TraceTypes.combine (ProofEntryT.internal StateT)))
+  (inferInstance: ErasableProofEntry (ExecTraceTypes.combine (ExecEntryT.internal StateT)) (ProofTraceTypes.combine (ProofEntryT.internal StateT)))
 
 public
-instance (StateT: Type): TraceTypes.HasStep (PersistentGlobalState.Compromise.ProofEntryT (LocalState StateT)) (ProofEntryT StateT) :=
-  inferInstanceAs (TraceTypes.HasStep (ProofEntryT.internal StateT 0) (TraceTypes.combine (ProofEntryT.internal StateT)))
+instance (StateT: Type): ProofTraceTypes.HasStep (PersistentGlobalState.Compromise.ProofEntryT (LocalState StateT)) (ProofEntryT StateT) :=
+  inferInstanceAs (ProofTraceTypes.HasStep (ProofEntryT.internal StateT 0) (ProofTraceTypes.combine (ProofEntryT.internal StateT)))
 
 public
-instance [TraceTypes] (StateT: Type): ∀ id, SubTraceInvariant (ProofEntryT.internal StateT id)
+instance [ExecTraceTypes] [ProofTraceTypes] (StateT: Type): ∀ id, SubTraceInvariant (ProofEntryT.internal StateT id)
   | 0 => by dsimp only [ProofEntryT.internal]; infer_instance
 
 public
-instance [TraceTypes] (StateT: Type): SubTraceInvariant (ProofEntryT StateT) :=
-  (inferInstance: SubTraceInvariant (TraceTypes.combine (ProofEntryT.internal StateT)))
+instance [ExecTraceTypes] [ProofTraceTypes] (StateT: Type): SubTraceInvariant (ProofEntryT StateT) :=
+  (inferInstance: SubTraceInvariant (ProofTraceTypes.combine (ProofEntryT.internal StateT)))
 
 public
-instance [TraceTypes] (StateT: Type): TraceInvariant.HasStep (PersistentGlobalState.Compromise.ProofEntryT (LocalState StateT)) (ProofEntryT StateT) :=
-  inferInstanceAs (TraceInvariant.HasStep (ProofEntryT.internal StateT 0) (TraceTypes.combine (ProofEntryT.internal StateT)))
+instance [ExecTraceTypes] [ProofTraceTypes] (StateT: Type): TraceInvariant.HasStep (PersistentGlobalState.Compromise.ProofEntryT (LocalState StateT)) (ProofEntryT StateT) :=
+  inferInstanceAs (TraceInvariant.HasStep (ProofEntryT.internal StateT 0) (ProofTraceTypes.combine (ProofEntryT.internal StateT)))
 
 public
 instance
-  [TraceInvariant] [BytesFunctor] [BytesInvariants]
+  [ExecTraceTypes] [ProofTraceTypes] [TraceInvariant] [BytesFunctor] [BytesInvariants]
   (StateT: Type)
-  [TraceTypes.Has (ProofEntryT StateT)]
+  [ExecTraceTypes.Has (ExecEntryT StateT)]
+  [ProofTraceTypes.Has (ProofEntryT StateT)]
   [TraceInvariant.Has (ProofEntryT StateT)]
   : ∀ id, SubBaseAttackerKnowledgeTheorem (ProofEntryT.internal StateT id) (baseAttackerKnowledge.internal StateT id)
   -- TODO: investigate why infer_instance doesn't work
@@ -344,9 +347,10 @@ instance
 
 public
 instance baseAttackerKnowledgeTheorem
-  [TraceInvariant] [BytesFunctor] [BytesInvariants]
+  [ExecTraceTypes] [ProofTraceTypes] [TraceInvariant] [BytesFunctor] [BytesInvariants]
   (StateT: Type)
-  [TraceTypes.Has (ProofEntryT StateT)]
+  [ExecTraceTypes.Has (ExecEntryT StateT)]
+  [ProofTraceTypes.Has (ProofEntryT StateT)]
   [TraceInvariant.Has (ProofEntryT StateT)]
   : SubBaseAttackerKnowledgeTheorem (ProofEntryT StateT) (baseAttackerKnowledge StateT)
 := by
@@ -378,7 +382,7 @@ grind_pattern label_isCorrupt => (label participant state).isCorrupt tr
 public
 class CompromisableLocalStateInv
   (StateT: Type)
-  [TraceTypes]
+  [ExecTraceTypes] [ProofTraceTypes]
   [BytesFunctor] [BytesInvariants]
   [BytesLength]
   [BytesFunctor.Has Literal.SubF] [BytesLength.Has Literal.SubF.length]
@@ -394,7 +398,7 @@ where
       Comparse.IsWellFormed (Bytes.KnowableBy (label participant state)) state tr
 
 instance
-  [TraceTypes] [BytesFunctor] [BytesInvariants]
+  [ExecTraceTypes] [ProofTraceTypes] [BytesFunctor] [BytesInvariants]
   [BytesLength]
   [BytesFunctor.Has Literal.SubF] [BytesLength.Has Literal.SubF.length] [BytesInvariants.Has Literal.invariants]
   [BytesFunctor.Has Concat.SubF] [BytesLength.Has Concat.SubF.length] [BytesInvariants.Has Concat.invariants]
@@ -419,10 +423,13 @@ theorem compromise.spec
   [BytesFunctor.Has Literal.SubF] [BytesLength.Has Literal.SubF.length]
   [BytesFunctor.Has Concat.SubF] [BytesLength.Has Concat.SubF.length]
   [Comparse.ParseableSerializeable StateT]
-  [TraceInvariant]
-  [TraceTypes.Has Network.ProofEntryT]
-  [TraceTypes.Has (State.ProofEntryT StateT)]
-  [TraceTypes.Has (Compromise.ProofEntryT StateT)]
+  [ExecTraceTypes] [ProofTraceTypes] [TraceInvariant]
+  [ExecTraceTypes.Has Network.ExecEntryT]
+  [ProofTraceTypes.Has Network.ProofEntryT]
+  [ExecTraceTypes.Has (State.ExecEntryT StateT)]
+  [ProofTraceTypes.Has (State.ProofEntryT StateT)]
+  [ExecTraceTypes.Has (Compromise.ExecEntryT StateT)]
+  [ProofTraceTypes.Has (Compromise.ProofEntryT StateT)]
   [BytesInvariants] [BytesInvariantsProofs]
   [BytesInvariants.Has Literal.invariants]
   [BytesInvariants.Has Concat.invariants]
@@ -487,7 +494,7 @@ def ProofEntryT.internal (StateT: Type): Fin 2 → Type
 @[expose, implicit_reducible]
 public
 def ProofEntryT (StateT: Type): Type :=
-  TraceTypes.combine (ProofEntryT.internal StateT)
+  ProofTraceTypes.combine (ProofEntryT.internal StateT)
 
 public
 instance (StateT: Type): ∀ id, ErasableProofEntry (ExecEntryT.internal StateT id) (ProofEntryT.internal StateT id)
@@ -495,19 +502,19 @@ instance (StateT: Type): ∀ id, ErasableProofEntry (ExecEntryT.internal StateT 
 
 public
 instance (StateT: Type): ErasableProofEntry (ExecEntryT StateT) (ProofEntryT StateT) :=
-  (inferInstance: ErasableProofEntry (ExecTraceTypes.combine (ExecEntryT.internal StateT)) (TraceTypes.combine (ProofEntryT.internal StateT)))
+  (inferInstance: ErasableProofEntry (ExecTraceTypes.combine (ExecEntryT.internal StateT)) (ProofTraceTypes.combine (ProofEntryT.internal StateT)))
 
 public
-instance (StateT: Type): TraceTypes.HasStep (State.ProofEntryT StateT) (ProofEntryT StateT) :=
-  inferInstanceAs (TraceTypes.HasStep (ProofEntryT.internal StateT 0) (TraceTypes.combine (ProofEntryT.internal StateT)))
+instance (StateT: Type): ProofTraceTypes.HasStep (State.ProofEntryT StateT) (ProofEntryT StateT) :=
+  inferInstanceAs (ProofTraceTypes.HasStep (ProofEntryT.internal StateT 0) (ProofTraceTypes.combine (ProofEntryT.internal StateT)))
 
 public
-instance (StateT: Type): TraceTypes.HasStep (Compromise.ProofEntryT StateT) (ProofEntryT StateT) :=
-  inferInstanceAs (TraceTypes.HasStep (ProofEntryT.internal StateT 1) (TraceTypes.combine (ProofEntryT.internal StateT)))
+instance (StateT: Type): ProofTraceTypes.HasStep (Compromise.ProofEntryT StateT) (ProofEntryT StateT) :=
+  inferInstanceAs (ProofTraceTypes.HasStep (ProofEntryT.internal StateT 1) (ProofTraceTypes.combine (ProofEntryT.internal StateT)))
 
 public
 instance
-  [TraceTypes] [BytesFunctor] [BytesInvariants]
+  [ExecTraceTypes] [ProofTraceTypes] [BytesFunctor] [BytesInvariants]
   [BytesLength] [BytesFunctor.Has Literal.SubF] [BytesLength.Has Literal.SubF.length] [BytesFunctor.Has Concat.SubF] [BytesLength.Has Concat.SubF.length]
   (StateT: Type) [Comparse.ParseableSerializeable StateT] [ExecTraceTypes.Has (ExecEntryT StateT)]
   [CompromisableLocalStateInv StateT]
@@ -516,40 +523,41 @@ instance
 
 public
 instance
-  [TraceTypes] [BytesFunctor] [BytesInvariants]
+  [ExecTraceTypes] [ProofTraceTypes] [BytesFunctor] [BytesInvariants]
   [BytesLength] [BytesFunctor.Has Literal.SubF] [BytesLength.Has Literal.SubF.length] [BytesFunctor.Has Concat.SubF] [BytesLength.Has Concat.SubF.length]
   (StateT: Type) [Comparse.ParseableSerializeable StateT] [ExecTraceTypes.Has (ExecEntryT StateT)]
   [CompromisableLocalStateInv StateT]
   : SubTraceInvariant (ProofEntryT StateT)
 :=
-  (inferInstance: SubTraceInvariant (TraceTypes.combine (ProofEntryT.internal StateT)))
+  (inferInstance: SubTraceInvariant (ProofTraceTypes.combine (ProofEntryT.internal StateT)))
 
 public
 instance
-  [TraceTypes] [BytesFunctor] [BytesInvariants]
+  [ExecTraceTypes] [ProofTraceTypes] [BytesFunctor] [BytesInvariants]
   [BytesLength] [BytesFunctor.Has Literal.SubF] [BytesLength.Has Literal.SubF.length] [BytesFunctor.Has Concat.SubF] [BytesLength.Has Concat.SubF.length]
   (StateT: Type) [Comparse.ParseableSerializeable StateT] [ExecTraceTypes.Has (ExecEntryT StateT)]
   [CompromisableLocalStateInv StateT]
   : TraceInvariant.HasStep (State.ProofEntryT StateT) (ProofEntryT StateT)
 :=
-  inferInstanceAs (TraceInvariant.HasStep (ProofEntryT.internal StateT 0) (TraceTypes.combine (ProofEntryT.internal StateT)))
+  inferInstanceAs (TraceInvariant.HasStep (ProofEntryT.internal StateT 0) (ProofTraceTypes.combine (ProofEntryT.internal StateT)))
 
 public
 instance
-  [TraceTypes] [BytesFunctor] [BytesInvariants]
+  [ExecTraceTypes] [ProofTraceTypes] [BytesFunctor] [BytesInvariants]
   [BytesLength] [BytesFunctor.Has Literal.SubF] [BytesLength.Has Literal.SubF.length] [BytesFunctor.Has Concat.SubF] [BytesLength.Has Concat.SubF.length]
   (StateT: Type) [Comparse.ParseableSerializeable StateT] [ExecTraceTypes.Has (ExecEntryT StateT)]
   [CompromisableLocalStateInv StateT]
   : TraceInvariant.HasStep (Compromise.ProofEntryT StateT) (ProofEntryT StateT)
 :=
-  inferInstanceAs (TraceInvariant.HasStep (ProofEntryT.internal StateT 1) (TraceTypes.combine (ProofEntryT.internal StateT)))
+  inferInstanceAs (TraceInvariant.HasStep (ProofEntryT.internal StateT 1) (ProofTraceTypes.combine (ProofEntryT.internal StateT)))
 
 public
 instance
-  [TraceInvariant] [BytesFunctor] [BytesInvariants]
+  [ExecTraceTypes] [ProofTraceTypes] [TraceInvariant] [BytesFunctor] [BytesInvariants]
   [BytesLength] [BytesFunctor.Has Literal.SubF] [BytesLength.Has Literal.SubF.length] [BytesFunctor.Has Concat.SubF] [BytesLength.Has Concat.SubF.length]
   (StateT: Type) [Comparse.ParseableSerializeable StateT]
-  [TraceTypes.Has (ProofEntryT StateT)]
+  [ExecTraceTypes.Has (ExecEntryT StateT)]
+  [ProofTraceTypes.Has (ProofEntryT StateT)]
   [CompromisableLocalStateInv StateT]
   [TraceInvariant.Has (ProofEntryT StateT)]
   : ∀ id, SubBaseAttackerKnowledgeTheorem (ProofEntryT.internal StateT id) (baseAttackerKnowledge.internal StateT id)
@@ -559,10 +567,11 @@ instance
 
 public
 instance baseAttackerKnowledgeTheorem
-  [TraceInvariant] [BytesFunctor] [BytesInvariants]
+  [ExecTraceTypes] [ProofTraceTypes] [TraceInvariant] [BytesFunctor] [BytesInvariants]
   [BytesLength] [BytesFunctor.Has Literal.SubF] [BytesLength.Has Literal.SubF.length] [BytesFunctor.Has Concat.SubF] [BytesLength.Has Concat.SubF.length]
   (StateT: Type) [Comparse.ParseableSerializeable StateT]
-  [TraceTypes.Has (ProofEntryT StateT)]
+  [ExecTraceTypes.Has (ExecEntryT StateT)]
+  [ProofTraceTypes.Has (ProofEntryT StateT)]
   [CompromisableLocalStateInv StateT]
   [TraceInvariant.Has (ProofEntryT StateT)]
   : SubBaseAttackerKnowledgeTheorem (ProofEntryT StateT) (baseAttackerKnowledge StateT)
