DY/Trace/Invariant.lean
@@ -15,25 +15,28 @@ abbrev ErasableProofEntry.default (ExecEntryT: Type): ErasableProofEntry ExecEnt
   erase x := x
 
 public
-class TraceTypes extends ExecTraceTypes where
+class ExecEntryAssociatedWithProofEntry (ExecEntryT: Type) (ProofEntryT: outParam Type) where
+
+public
+class ProofTraceTypes [ExecTraceTypes] where
   ProofT: Type
-  tc: ErasableProofEntry ExecT ProofT
+  tc: ErasableProofEntry ExecTraceTypes.ExecT ProofT
 
 @[expose]
 public
-def ProofTrace.Entry [TraceTypes] := TraceTypes.ProofT
+def ProofTrace.Entry [ExecTraceTypes] [ProofTraceTypes] := ProofTraceTypes.ProofT
 
 public
-instance [TraceTypes]: ErasableProofEntry ExecTrace.Entry ProofTrace.Entry where
-  erase entry := TraceTypes.tc.erase entry
+instance [ExecTraceTypes] [ProofTraceTypes]: ErasableProofEntry ExecTrace.Entry ProofTrace.Entry where
+  erase entry := ProofTraceTypes.tc.erase entry
 
 public
-abbrev ProofTrace [TraceTypes] := Trace ProofTrace.Entry
+abbrev ProofTrace [ExecTraceTypes] [ProofTraceTypes] := Trace ProofTrace.Entry
 
 @[expose]
 public
 def ProofTrace.Entry.erase
-  [TraceTypes]
+  [ExecTraceTypes] [ProofTraceTypes]
   (entry: ProofTrace.Entry)
   : ExecTrace.Entry
 :=
@@ -41,7 +44,7 @@ def ProofTrace.Entry.erase
 
 public
 def Trace.erase
-  [TraceTypes]
+  [ExecTraceTypes] [ProofTraceTypes]
   (tr: ProofTrace)
   : ExecTrace
 :=
@@ -51,7 +54,7 @@ def Trace.erase
 
 public
 theorem Trace.erase_le
-  [TraceTypes]
+  [ExecTraceTypes] [ProofTraceTypes]
   (tr1 tr2: ProofTrace)
   : tr1 ≤ tr2 →
     tr1.erase ≤ tr2.erase
@@ -67,7 +70,7 @@ grind_pattern [grind_later] Trace.erase_le => tr1 ≤ tr2, tr1.erase
 
 public
 theorem Trace.erase_length
-  [TraceTypes]
+  [ExecTraceTypes] [ProofTraceTypes]
   (tr: ProofTrace)
   : tr.erase.length = tr.length
 := by
@@ -78,7 +81,7 @@ grind_pattern Trace.erase_length => tr.erase.length
 
 public
 def Trace.erase_at
-  [TraceTypes]
+  [ExecTraceTypes] [ProofTraceTypes]
   (tr: ProofTrace)
   (i: Nat) (h_i: i < tr.erase.length)
   : tr.erase.at i h_i = (tr.at i (Trace.erase_length tr ▸ h_i)).erase
@@ -90,40 +93,40 @@ def Trace.erase_at
   grind [Trace.erase_length]
 
 -- TODO test coercion
-example [TraceTypes]: Coe ProofTrace ExecTrace where
+example [ExecTraceTypes] [ProofTraceTypes]: Coe ProofTrace ExecTrace where
   coe tr := tr.erase
 
 public
-class TraceTypes.Has
-  [TraceTypes]
+class ProofTraceTypes.Has
+  [ExecTraceTypes] [ProofTraceTypes]
   {ExecEntryT: outParam Type} (ProofEntryT: Type)
   [ErasableProofEntry ExecEntryT ProofEntryT]
-  extends ExecTraceTypes.Has ExecEntryT
+  [ExecTraceTypes.Has ExecEntryT]
 where
   proofInj: ProofEntryT → ProofTrace.Entry
   proofProj: ProofTrace.Entry → Option ProofEntryT
   proof_inj_proj_eq: ∀ x y, (proofProj x = some y) = (x = proofInj y)
-  proofProj_none_eq_erase: ∀ x, ((proofProj x: Option ProofEntryT) = none) = ((proj x.erase: Option ExecEntryT) = none)
-  erase_commutes: ∀ entry, (proofInj entry).erase = inj (ErasableProofEntry.erase entry)
+  proofProj_none_eq_erase: ∀ x, ((proofProj x: Option ProofEntryT) = none) = ((ExecTraceTypes.Has.proj x.erase: Option ExecEntryT) = none)
+  erase_commutes: ∀ entry, (proofInj entry).erase = ExecTraceTypes.Has.inj (ErasableProofEntry.erase entry)
 
 public
-class TraceTypes.HasStep
+class ProofTraceTypes.HasStep
   {ExecEntryT1 ExecEntryT2: outParam Type}
   (ProofEntryT1: Type) (ProofEntryT2: semiOutParam Type)
   [ErasableProofEntry ExecEntryT1 ProofEntryT1]
   [ErasableProofEntry ExecEntryT2 ProofEntryT2]
-  extends ExecTraceTypes.HasStep ExecEntryT1 ExecEntryT2
+  [ExecTraceTypes.HasStep ExecEntryT1 ExecEntryT2]
 where
   proofInj: ProofEntryT1 → ProofEntryT2
   proofProj: ProofEntryT2 → Option ProofEntryT1
   proof_inj_proj_eq: ∀ x y, (proofProj x = some y) = (x = proofInj y)
-  proofProj_none_eq_erase: ∀ x, ((proofProj x: Option ProofEntryT1) = none) = ((proj (ErasableProofEntry.erase x): Option ExecEntryT1) = none)
-  erase_commutes: ∀ entry, ErasableProofEntry.erase (proofInj entry) = inj (ErasableProofEntry.erase entry)
+  proofProj_none_eq_erase: ∀ x, ((proofProj x: Option ProofEntryT1) = none) = ((ExecTraceTypes.HasStep.proj (ErasableProofEntry.erase x): Option ExecEntryT1) = none)
+  erase_commutes: ∀ entry, ErasableProofEntry.erase (proofInj entry) = ExecTraceTypes.HasStep.inj (ErasableProofEntry.erase entry)
 
 public
-instance instTraceTypesHasItself
-  [TraceTypes]
-  : TraceTypes.Has ProofTrace.Entry
+instance instProofTraceTypesHasItself
+  [ExecTraceTypes] [ProofTraceTypes]
+  : ProofTraceTypes.Has ProofTrace.Entry
 where
   proofInj entry := entry
   proofProj entry := some entry
@@ -132,47 +135,56 @@ where
   erase_commutes := by simp [ExecTraceTypes.Has.inj, ProofTrace.Entry.erase]
 
 public
-instance instTraceTypesHasStep
-  [TraceTypes]
+instance instProofTraceTypesHasStep
+  [ExecTraceTypes] [ProofTraceTypes]
   {ExecEntryT1 ExecEntryT2: Type}
   (ProofEntryT1 ProofEntryT2: Type)
   [ErasableProofEntry ExecEntryT1 ProofEntryT1]
   [ErasableProofEntry ExecEntryT2 ProofEntryT2]
-  [TraceTypes.HasStep ProofEntryT1 ProofEntryT2]
-  [TraceTypes.Has ProofEntryT2]
-  : TraceTypes.Has ProofEntryT1
+  [ExecTraceTypes.HasStep ExecEntryT1 ExecEntryT2]
+  [ProofTraceTypes.HasStep ProofEntryT1 ProofEntryT2]
+  [ExecTraceTypes.Has ExecEntryT2]
+  [ProofTraceTypes.Has ProofEntryT2]
+  : ProofTraceTypes.Has ProofEntryT1
 where
-  proofInj entry := TraceTypes.Has.proofInj (TraceTypes.HasStep.proofInj (ProofEntryT2 := ProofEntryT2) entry)
+  proofInj entry := ProofTraceTypes.Has.proofInj (ProofTraceTypes.HasStep.proofInj (ProofEntryT2 := ProofEntryT2) entry)
   proofProj entry :=
-    match TraceTypes.Has.proofProj (ProofEntryT := ProofEntryT2) entry with
+    match ProofTraceTypes.Has.proofProj (ProofEntryT := ProofEntryT2) entry with
     | none => none
-    | some y => TraceTypes.HasStep.proofProj y
+    | some y => ProofTraceTypes.HasStep.proofProj y
 
   proof_inj_proj_eq x y := by
-    have := TraceTypes.Has.proof_inj_proj_eq (ProofEntryT := ProofEntryT2) x
-    have := TraceTypes.HasStep.proof_inj_proj_eq (ProofEntryT1 := ProofEntryT1) (ProofEntryT2 := ProofEntryT2)
+    have := ProofTraceTypes.Has.proof_inj_proj_eq (ProofEntryT := ProofEntryT2) x
+    have := ProofTraceTypes.HasStep.proof_inj_proj_eq (ProofEntryT1 := ProofEntryT1) (ProofEntryT2 := ProofEntryT2)
     grind
   proofProj_none_eq_erase := by
     intro x
     have := ExecTraceTypes.Has.inj_proj_eq (ExecEntryT := ExecEntryT2)
-    have := TraceTypes.Has.proof_inj_proj_eq (ProofEntryT := ProofEntryT2)
-    have := TraceTypes.Has.proofProj_none_eq_erase (ProofEntryT := ProofEntryT2)
-    have := TraceTypes.HasStep.proofProj_none_eq_erase (ProofEntryT1 := ProofEntryT1) (ProofEntryT2 := ProofEntryT2)
-    have := TraceTypes.Has.erase_commutes (ProofEntryT := ProofEntryT2)
+    have := ProofTraceTypes.Has.proof_inj_proj_eq (ProofEntryT := ProofEntryT2)
+    have := ProofTraceTypes.Has.proofProj_none_eq_erase (ProofEntryT := ProofEntryT2)
+    have := ProofTraceTypes.HasStep.proofProj_none_eq_erase (ProofEntryT1 := ProofEntryT1) (ProofEntryT2 := ProofEntryT2)
+    have := ProofTraceTypes.Has.erase_commutes (ProofEntryT := ProofEntryT2)
     simp [ExecTraceTypes.Has.proj]
     grind
   erase_commutes := by
-    have := TraceTypes.Has.erase_commutes (ProofEntryT := ProofEntryT2)
-    have := TraceTypes.HasStep.erase_commutes (ProofEntryT1 := ProofEntryT1) (ProofEntryT2 := ProofEntryT2)
+    have := ProofTraceTypes.Has.erase_commutes (ProofEntryT := ProofEntryT2)
+    have := ProofTraceTypes.HasStep.erase_commutes (ProofEntryT1 := ProofEntryT1) (ProofEntryT2 := ProofEntryT2)
     simp [ExecTraceTypes.Has.inj]
     grind
 
 public
-instance [TraceTypes] {ExecEntryT: Type} (ProofEntryT: Type) [ErasableProofEntry ExecEntryT ProofEntryT] [TraceTypes.Has ProofEntryT]: IntoTraceEntry ProofEntryT ProofTrace.Entry where
-  make entry := TraceTypes.Has.proofInj entry
+instance
+  [ExecTraceTypes] [ProofTraceTypes]
+  {ExecEntryT ProofEntryT: Type}
+  [ErasableProofEntry ExecEntryT ProofEntryT]
+  [ExecTraceTypes.Has ExecEntryT]
+  [ProofTraceTypes.Has ProofEntryT]
+  : IntoTraceEntry ProofEntryT ProofTrace.Entry
+where
+  make entry := ProofTraceTypes.Has.proofInj entry
 
 public
-structure TraceTypes.combine {n: Nat} (ProofTypes: Fin n → Type): Type where
+structure ProofTraceTypes.combine {n: Nat} (ProofTypes: Fin n → Type): Type where
   id: Fin n
   entry: ProofTypes id
 
@@ -182,18 +194,18 @@ instance
   (ExecTypes: Fin n → Type)
   (ProofTypes: Fin n → Type)
   [∀ id, ErasableProofEntry (ExecTypes id) (ProofTypes id)]
-  : ErasableProofEntry (ExecTraceTypes.combine ExecTypes) (TraceTypes.combine ProofTypes)
+  : ErasableProofEntry (ExecTraceTypes.combine ExecTypes) (ProofTraceTypes.combine ProofTypes)
 where
   erase := fun { id, entry } => { id, entry := ErasableProofEntry.erase entry }
 
 public
-instance instTraceTypesCombineHasStep
+instance instProofTraceTypesCombineHasStep
   {n: Nat}
   (ExecTypes: Fin n → Type)
   (ProofTypes: Fin n → Type)
   [∀ id, ErasableProofEntry (ExecTypes id) (ProofTypes id)]
   (id: Fin n):
-  TraceTypes.HasStep (ProofTypes id) (TraceTypes.combine ProofTypes)
+  ProofTraceTypes.HasStep (ProofTypes id) (ProofTraceTypes.combine ProofTypes)
 where
   proofInj entry := { id, entry }
   proofProj entry :=
@@ -210,88 +222,93 @@ where
 
 public
 theorem ProofTrace.Entry.erase_eq_imp_exists
-  [TraceTypes]
+  [ExecTraceTypes] [ProofTraceTypes]
   {ExecEntryT ProofEntryT: Type}
   [ErasableProofEntry ExecEntryT ProofEntryT]
-  [TraceTypes.Has ProofEntryT]
+  [ExecEntryAssociatedWithProofEntry ExecEntryT ProofEntryT]
+  [ExecTraceTypes.Has ExecEntryT]
+  [ProofTraceTypes.Has ProofEntryT]
   {entry: ProofTrace.Entry}
   {result: ExecEntryT}
   : entry.erase = ExecTraceTypes.Has.inj result ↔ (
       ∃ result': ProofEntryT,
-      entry = TraceTypes.Has.proofInj result' ∧
+      entry = ProofTraceTypes.Has.proofInj result' ∧
       ErasableProofEntry.erase result' = result
     )
 := by
-  cases h: (TraceTypes.Has.proofProj entry: Option ProofEntryT)
-  · have := TraceTypes.Has.proofProj_none_eq_erase (ProofEntryT := ProofEntryT) entry
+  cases h: (ProofTraceTypes.Has.proofProj entry: Option ProofEntryT)
+  · have := ProofTraceTypes.Has.proofProj_none_eq_erase (ProofEntryT := ProofEntryT) entry
     rewrite [← ExecTraceTypes.Has.inj_proj_eq]
     simp_all only [reduceCtorEq, false_iff, not_exists]
     intro x
-    have := TraceTypes.Has.proof_inj_proj_eq entry x
+    have := ProofTraceTypes.Has.proof_inj_proj_eq entry x
     grind
   · rename_i result'
-    rewrite [TraceTypes.Has.proof_inj_proj_eq] at h
-    grind [TraceTypes.Has.erase_commutes]
+    rewrite [ProofTraceTypes.Has.proof_inj_proj_eq] at h
+    grind [ProofTraceTypes.Has.erase_commutes]
 
 public
 theorem Trace.append_erase
-  [TraceTypes]
+  [ExecTraceTypes] [ProofTraceTypes]
   {ExecEntryT ProofEntryT: Type}
   [ErasableProofEntry ExecEntryT ProofEntryT]
-  [TraceTypes.Has ProofEntryT]
+  [ExecTraceTypes.Has ExecEntryT]
+  [ProofTraceTypes.Has ProofEntryT]
   (tr: ProofTrace) (entry: ProofEntryT)
   : (tr.append entry).erase = tr.erase.append (ErasableProofEntry.erase entry)
 := by
-  simp [Trace.append, Trace.erase, IntoTraceEntry.make, TraceTypes.Has.erase_commutes]
+  simp [Trace.append, Trace.erase, IntoTraceEntry.make, ProofTraceTypes.Has.erase_commutes]
 
 public
 theorem Trace.at_is_imp_proofProj_at
-  [TraceTypes]
+  [ExecTraceTypes] [ProofTraceTypes]
   {ExecEntryT ProofEntryT: Type}
   [ErasableProofEntry ExecEntryT ProofEntryT]
-  [TraceTypes.Has ProofEntryT]
+  [ExecTraceTypes.Has ExecEntryT]
+  [ProofTraceTypes.Has ProofEntryT]
   (tr: ProofTrace) (i: Nat) (entry: ProofEntryT)
   : tr.at_is i entry →
     exists h: i < tr.length,
-    TraceTypes.Has.proofProj (tr.at i h) = some entry
+    ProofTraceTypes.Has.proofProj (tr.at i h) = some entry
 := by
   simp only [Trace.at_is, IntoTraceEntry.make]
   intro ⟨ h1, h2 ⟩
   exists h1
-  grind [TraceTypes.Has.proof_inj_proj_eq]
+  grind [ProofTraceTypes.Has.proof_inj_proj_eq]
 
 public
 theorem Trace.at_is_erase
-  [TraceTypes]
+  [ExecTraceTypes] [ProofTraceTypes]
   {ExecEntryT ProofEntryT: Type}
   [ErasableProofEntry ExecEntryT ProofEntryT]
-  [TraceTypes.Has ProofEntryT]
+  [ExecTraceTypes.Has ExecEntryT]
+  [ProofTraceTypes.Has ProofEntryT]
   (tr: ProofTrace) (i: Nat) (entry: ProofEntryT)
   : tr.at_is i entry →
     tr.erase.at_is i (ErasableProofEntry.erase entry)
 := by
   simp only [Trace.at_is, IntoTraceEntry.make]
   intro ⟨ h1, h2 ⟩
-  simp_all [Trace.erase_at, TraceTypes.Has.erase_commutes]
+  simp_all [Trace.erase_at, ProofTraceTypes.Has.erase_commutes]
   grind
 
 -- Invariant
 
 public
-class SubTraceInvariant [TraceTypes] {ExecEntryT: outParam Type} (ProofEntryT: Type) [ErasableProofEntry ExecEntryT ProofEntryT] where
+class SubTraceInvariant [ExecTraceTypes] [ProofTraceTypes] {ExecEntryT: outParam Type} (ProofEntryT: Type) [ErasableProofEntry ExecEntryT ProofEntryT] where
   invariant: ProofTrace → ProofEntryT → Prop
 
 public
-class TraceInvariant extends TraceTypes where
+class TraceInvariant [ExecTraceTypes] [ProofTraceTypes] where
   tc_inv: SubTraceInvariant ProofTrace.Entry
 
 public
-instance [TraceInvariant]: SubTraceInvariant ProofTrace.Entry where
+instance [ExecTraceTypes] [ProofTraceTypes] [ExecTraceTypes] [ProofTraceTypes] [TraceInvariant]: SubTraceInvariant ProofTrace.Entry where
   invariant := TraceInvariant.tc_inv.invariant
 
 public
 def ProofTrace.Entry.Invariant
-  [TraceInvariant]
+  [ExecTraceTypes] [ProofTraceTypes] [TraceInvariant]
   (trBefore: ProofTrace)
   (entry: ProofTrace.Entry)
   : Prop
@@ -300,7 +317,7 @@ def ProofTrace.Entry.Invariant
 
 public
 def Trace.Invariant
-  [TraceInvariant]
+  [ExecTraceTypes] [ProofTraceTypes] [TraceInvariant]
   (tr: ProofTrace)
   : Prop
 :=
@@ -312,44 +329,48 @@ def Trace.Invariant
 
 public
 class TraceInvariant.Has
-  [TraceInvariant]
+  [ExecTraceTypes] [ProofTraceTypes] [TraceInvariant]
   {ExecEntryT: outParam Type}
   (ProofEntryT: Type)
   [ErasableProofEntry ExecEntryT ProofEntryT]
-  [TraceTypes.Has ProofEntryT]
+  [ExecTraceTypes.Has ExecEntryT]
+  [ProofTraceTypes.Has ProofEntryT]
   [SubTraceInvariant ProofEntryT]
 where
-  inv_commutes: ∀ trBefore: ProofTrace, ∀ entry: ProofEntryT, (TraceTypes.Has.proofInj entry).Invariant trBefore = SubTraceInvariant.invariant trBefore entry
+  inv_commutes: ∀ trBefore: ProofTrace, ∀ entry: ProofEntryT, (ProofTraceTypes.Has.proofInj entry).Invariant trBefore = SubTraceInvariant.invariant trBefore entry
 
 public
 class TraceInvariant.HasStep
-  [TraceTypes]
+  [ExecTraceTypes] [ProofTraceTypes]
   {ExecEntryT1 ExecEntryT2: outParam Type}
   (ProofEntryT1 ProofEntryT2: Type)
   [ErasableProofEntry ExecEntryT1 ProofEntryT1]
   [ErasableProofEntry ExecEntryT2 ProofEntryT2]
-  [TraceTypes.HasStep ProofEntryT1 ProofEntryT2]
+  [ExecTraceTypes.HasStep ExecEntryT1 ExecEntryT2]
+  [ProofTraceTypes.HasStep ProofEntryT1 ProofEntryT2]
   [SubTraceInvariant ProofEntryT1]
   [SubTraceInvariant ProofEntryT2]
 where
-  inv_commutes: ∀ trBefore: ProofTrace, ∀ entry: ProofEntryT1, SubTraceInvariant.invariant trBefore (TraceTypes.HasStep.proofInj entry: ProofEntryT2) = SubTraceInvariant.invariant trBefore entry
+  inv_commutes: ∀ trBefore: ProofTrace, ∀ entry: ProofEntryT1, SubTraceInvariant.invariant trBefore (ProofTraceTypes.HasStep.proofInj entry: ProofEntryT2) = SubTraceInvariant.invariant trBefore entry
 
 public
 instance instTraceInvariantHasItself
-  [TraceInvariant]
+  [ExecTraceTypes] [ProofTraceTypes] [TraceInvariant]
   : TraceInvariant.Has ProofTrace.Entry
 where
-  inv_commutes := by simp [TraceTypes.Has.proofInj, ProofTrace.Entry.Invariant]
+  inv_commutes := by simp [ProofTraceTypes.Has.proofInj, ProofTrace.Entry.Invariant]
 
 public
 instance instTraceInvariantHasStep
-  [TraceInvariant]
+  [ExecTraceTypes] [ProofTraceTypes] [TraceInvariant]
   {ExecEntryT1 ProofEntryT1: Type}
   {ExecEntryT2 ProofEntryT2: Type}
   [ErasableProofEntry ExecEntryT1 ProofEntryT1]
   [ErasableProofEntry ExecEntryT2 ProofEntryT2]
-  [TraceTypes.HasStep ProofEntryT1 ProofEntryT2]
-  [TraceTypes.Has ProofEntryT2]
+  [ExecTraceTypes.HasStep ExecEntryT1 ExecEntryT2]
+  [ProofTraceTypes.HasStep ProofEntryT1 ProofEntryT2]
+  [ExecTraceTypes.Has ExecEntryT2]
+  [ProofTraceTypes.Has ProofEntryT2]
   [SubTraceInvariant ProofEntryT1]
   [SubTraceInvariant ProofEntryT2]
   [TraceInvariant.HasStep ProofEntryT1 ProofEntryT2]
@@ -359,40 +380,41 @@ where
   inv_commutes := by
     have := TraceInvariant.HasStep.inv_commutes (ProofEntryT1 := ProofEntryT1) (ProofEntryT2 := ProofEntryT2)
     have := TraceInvariant.Has.inv_commutes (ProofEntryT := ProofEntryT2)
-    simp_all [TraceTypes.Has.proofInj]
+    simp_all [ProofTraceTypes.Has.proofInj]
 
 public
 instance SubTraceInvariant.combine
-  [TraceTypes]
+  [ExecTraceTypes] [ProofTraceTypes]
   {n: Nat}
   {ExecTypes: Fin n → Type}
   {ProofTypes: Fin n → Type}
   [∀ id, ErasableProofEntry (ExecTypes id) (ProofTypes id)]
   [∀ id, SubTraceInvariant (ProofTypes id)]
-  : SubTraceInvariant (TraceTypes.combine ProofTypes)
+  : SubTraceInvariant (ProofTraceTypes.combine ProofTypes)
 where
   invariant := fun trBefore { id := _, entry } =>
     SubTraceInvariant.invariant trBefore entry
 
 public
 instance instTraceInvariantCombineHasStep
-  [TraceTypes]
+  [ExecTraceTypes] [ProofTraceTypes]
   {n: Nat}
   {ExecTypes: Fin n → Type}
   (ProofTypes: Fin n → Type)
   [∀ id, ErasableProofEntry (ExecTypes id) (ProofTypes id)]
   [∀ id, SubTraceInvariant (ProofTypes id)]
   (id: Fin n)
-  : TraceInvariant.HasStep (ProofTypes id) (TraceTypes.combine ProofTypes)
+  : TraceInvariant.HasStep (ProofTypes id) (ProofTraceTypes.combine ProofTypes)
 where
   inv_commutes trBefore entry := by rfl
 
 public
 theorem Trace.invariant_append
-  [TraceInvariant]
+  [ExecTraceTypes] [ProofTraceTypes] [TraceInvariant]
   {ExecEntryT ProofEntryT: Type}
   [ErasableProofEntry ExecEntryT ProofEntryT]
-  [TraceTypes.Has ProofEntryT]
+  [ExecTraceTypes.Has ExecEntryT]
+  [ProofTraceTypes.Has ProofEntryT]
   [SubTraceInvariant ProofEntryT]
   [TraceInvariant.Has ProofEntryT]
   (tr: ProofTrace) (entry: ProofEntryT)
@@ -403,7 +425,7 @@ theorem Trace.invariant_append
 
 public
 theorem Trace.invariant_at
-  [TraceInvariant]
+  [ExecTraceTypes] [ProofTraceTypes] [TraceInvariant]
   (tr: ProofTrace)
   (i: Nat)
   (h_i: i < tr.length)
