DY/EquationalTheory/Literal.lean
@@ -138,7 +138,7 @@ end AttackerKnowledge
 
 section Invariants
 
-variable [TraceTypes]
+variable [ExecTraceTypes] [ProofTraceTypes]
 variable [BytesFunctor] [BytesFunctor.Has SubF]
 
 public
@@ -194,7 +194,7 @@ end Invariants
 
 section AttackerKnowledgeTheorem
 
-variable [TraceInvariant]
+variable [ExecTraceTypes] [ProofTraceTypes] [TraceInvariant]
 variable [BytesFunctor] [BytesInvariants]
 variable [BytesFunctor.Has SubF]
 variable [BytesInvariants.Has invariants]
